Made code look nice for the video

TCR/Data/SegmentTree/Basic.lean
@@ -6,6 +6,7 @@ Authors: Markus Himmel
 module
 
 public import TCR.Data.Vector
+import TCR.Data.SegmentTree.Lies
 
 /-!
 # Segment trees
@@ -20,71 +21,82 @@ namespace Impl
 
 /-- A vector of size `2 * n` is an `op`-segment tree if, when interpreted as a binary tree,
 it satisfies the heap-like property that the parent is always the `op` of the children. -/
-public structure IsSegmentTree (op : α → α → α) (neutral : α) (v : Vector α (2 * n)) : Prop where
+public structure IsSegmentTree (op : α → α → α) (neutral : α) (v : Vector α (n + n)) : Prop where
   /-- The unused zero-th element of `v` is the neutral element, to ensure that segment trees on
   a given underlying array are unique. -/
-  zero_eq : ∀ (h : 0 < 2 * n), v[0] = neutral
+  zero_eq : ∀ (h : 0 < n + n), v[0] = neutral
   /-- Given `0 < i < n`, `v[i] = op v[2 * i] v[2 * i + 1]`, i.e., a node stores the combination of its children. -/
   op_eq : ∀ (i : Nat) (_ : 0 < i) (hi : i < n), v[i] = op v[2 * i] v[2 * i + 1]
 
-macro_rules
-  | `(tactic| get_elem_tactic_extensible) => `(tactic| grind)
-
-/-- Creates a new `op`-segment tree on the vector `v`. -/
-@[inline]
-def mkSegmentTree (op : α → α → α) (neutral : α) (v : Vector α n) : Vector α (2 * n) :=
-  if h : n = 0 then
-    Vector.mk #[] (by grind)
-  else
-    let vec := Vector.mk (Array.replicate n neutral ++ v.toArray) (by grind)
-    loop vec (n - 1)
+/-- Creates a new `op`-segment tree on the vector `a`. -/
+def mkSegmentTree (op : α → α → α) (neutral : α) (a : Vector α n) (h : 0 < n) : Vector α (n + n) :=
+  let v := Vector.replicate n neutral ++ a
+  loop v (n - 1)  
 where
-  @[specialize] loop (vec : Vector α (2 * n)) (idx : Nat) (hidx : idx < n := by grind) : Vector α (2 * n) :=
-    match h : idx with
-    | 0 => vec
-    | _ + 1 => loop (vec.set idx (op vec[2 * idx] vec[2 * idx + 1])) (idx - 1)
+  loop (v : Vector α (n + n)) (idx : Nat) (hidx : idx < n) : Vector α (n + n) :=
+    if h : idx = 0 then
+      v
+    else
+      loop (v.set idx (op v[2 * idx] v[2 * idx + 1])) (idx - 1)  
 
-/-- Creates an empty segment tree using the neutral element `neutral`. -/
-@[inline]
-def mkEmpty (neutral : α) (n : Nat) : Vector α (2 * n) :=
-  Vector.replicate (2 * n) neutral
+def mkSegmentTree' (op : α → α → α) (neutral : α) (a : Vector α n) : Vector α (n + n) :=
+  if h : n = 0 then
+    Vector.mk #[] (by simp [h])
+  else
+    mkSegmentTree op neutral a (by grind)
 
-/-- Given a segment tree, extracts the underlying data by copying it. -/
-@[inline]
-def underlying (v : Vector α (2 * n)) : Vector α n :=
-  v.extract n (2 * n) |>.cast <| by grind
+/-- Updates the segment tree to have value `a` at index `i`. -/
+def update (op : α → α → α) (v : Vector α (n + n)) (i : Nat) (hi : i < n) (a : α) : Vector α (n + n) :=
+  loop (v.set (n + i) a) ((n + i) / 2)  
+where
+  loop (vec : Vector α (n + n)) (idx : Nat) (h : idx < n) : Vector α (n + n) :=
+    if h : idx = 0 then
+      vec
+    else
+      loop (vec.set idx (op vec[2 * idx] vec[2 * idx + 1])) (idx / 2)  
 
 /-- Modifies the underlying array of the segment tree at position `i` using
 `f` and restores the segment tree property. -/
 @[inline]
-def modify (op : α → α → α) (v : Vector α (2 * n)) (i : Nat) (hi : i < n) (f : α → α) : Vector α (2 * n) :=
+def modify (op : α → α → α) (v : Vector α (n + n)) (i : Nat) (hi : i < n) (f : α → α) : Vector α (n + n) :=
   loop (v.modify (n + i) f) ((n + i) / 2)
 where
-  @[specialize] loop (vec : Vector α (2 * n)) (idx : Nat) (h : idx < n := by grind) : Vector α (2 * n) :=
+  @[specialize] loop (vec : Vector α (n + n)) (idx : Nat) (h : idx < n := by grind) : Vector α (n + n) :=
     if h : idx = 0 then
       vec
     else
       loop (vec.set idx (op vec[2 * idx] vec[2 * idx + 1])) (idx / 2)
 
-/-- Folds the operation over `underlying[l...<r]`. -/
+/-- Creates an empty segment tree using the neutral element `neutral`. -/
 @[inline]
-def query (op : α → α → α) (neutral : α) (v : Vector α (2 * n)) (l r : Nat) (hlr : l ≤ r) (hr : r ≤ n) : α :=
-  loop (l + n) (r + n) neutral neutral
+def mkEmpty (neutral : α) (n : Nat) : Vector α (n + n) :=
+  Vector.replicate (n + n) neutral
+
+/-- Given a segment tree, extracts the underlying data by copying it. -/
+@[inline]
+def underlying (v : Vector α (n + n)) : Vector α n :=
+  v.extract n (n + n) |>.cast <| by grind
+
+/-- Folds the operation over `underlying[l₀...<r₀]`. -/
+@[inline]
+def query (op : α → α → α) (neutral : α) (v : Vector α (n + n)) (l₀ r₀ : Nat)
+    (hlr : l₀ ≤ r₀) (hr : r₀ ≤ n) : α :=
+  loop (l₀ + n) (r₀ + n) neutral neutral  
 where
-  @[specialize] loop (l r : Nat) (resl resr : α) (h : l ≤ r ∧ r ≤ 2 * n := by grind) : α :=
-    if h : l < r then
+  loop (l r : Nat) (resl resr : α) (h : l ≤ r ∧ r ≤ 2 * n) : α :=
+    𝚒f l < r then
       let resl := if l % 2 = 0 then resl else op resl v[l]
       let resr := if r % 2 = 0 then resr else op v[r - 1] resr
-      loop ((l + 1) / 2) (r / 2) resl resr
+      loop ((l + 1) / 2) (r / 2) resl resr  
     else
       op resl resr
 
 /-- Inductive well-formedness predicate for segment trees. In `TCR.Data.SegmentTree.WF` we show that the first
 constructors subsumes all other ones, i.e., that all operations preserve the segment tree property, see
 `Impl.WF.out`. -/
-public protected inductive WF (op : α → α → α) (neutral : α) : Vector α (2 * n) → Prop where
+public protected inductive WF (op : α → α → α) (neutral : α) : Vector α (n + n) → Prop where
   | isSegmentTree : IsSegmentTree op neutral v → Impl.WF op neutral v
-  | private mkSegmentTree : Impl.WF op neutral (mkSegmentTree op neutral v)
+  | private mkSegmentTree : Impl.WF op neutral (mkSegmentTree' op neutral v)
   | private mkEmpty : Impl.WF op neutral (mkEmpty neutral n)
   | private modify : Impl.WF op neutral v → Impl.WF op neutral (modify op v i hi f)
 
@@ -98,14 +110,14 @@ This is an efficient implementation representing the segment tree as an implicit
 array. As with all data structures based on arrays, care should be taken to use it linearly. -/
 public structure _root_.TCR.SegmentTree (op : α → α → α) (neutral : α) (n : Nat) where
   /-- The segment tree, stored as an implicit binary tree. -/
-  tree : Vector α (2 * n)
+  tree : Vector α (n + n)
   /-- The tree forms a valid segment tree. -/
   wf : Impl.WF op neutral tree
 
 /-- Constructs an `op`-segment tree from the vector `v.` -/
 @[inline]
 public def ofVector (op : α → α → α) (neutral : α) (v : Vector α n) : SegmentTree op neutral n where
-  tree := Impl.mkSegmentTree op neutral v
+  tree := Impl.mkSegmentTree' op neutral v
   wf := .mkSegmentTree
 
 /-- Constructs an empty `op`-segment tree whose underlying array has size `n`. -/
