TCR/Data/SegmentTree/Lies.lean
@@ -1,0 +1,26 @@
+module
+
+/-!
+Welcome to `Lies.lean`, where we use Lean's syntax extensibility to make
+Lean look nice for the video. There are two hacks:
+
+* We override the `if` syntax so that `if P then Q else R` expands to
+  `if _ : P then Q else R`, which introduces the hypothesis `P` or `¬P`
+  into the context for automation we use. Actually, we define a new
+  syntax `𝚒f` which is completely separate from the usual `if`. Yes,
+  you saw that right, that is `i` as in `U+1D692 Mathematical Monospace Small I`.
+* We define ` ` as in `U+2009 Thin Space` to mean `by grind`, so that
+  automation calls become invisible.
+-/
+
+macro " ": term => `(term|by grind)
+
+syntax
+  ppRealGroup(ppRealFill(ppIndent("𝚒f " term " then") ppSpace term)
+    ppDedent(ppSpace) ppRealFill("else " term)) : term
+
+macro_rules
+  | `(𝚒f $c then $t else $e) => `(if _ : $c then $t else $e)
+
+macro_rules
+  | `(tactic| get_elem_tactic_extensible) => `(tactic| grind)
